SystemFD/Examples/Maybe.lean
@@ -11,27 +11,8 @@ def MaybeBoolCtx : Ctx Term := [
          Λ u. λ (tmu : t ~ Maybe u). λ eqU : Eq u.
            eqMaybe ▹ sym (<t ~ Bool> → <t ~ Bool> → <Bool>)
     -/
-    .inst 8 (Λ[★] `λ[#10 `@k #0] -- Λt. λ(i : Eq t)
-                   .guard (#3 `@t #1) #0    --     EqMaybe[t] ← i
-                    (Λ[★] `λ[#2 ~ (#7 `@k #0)] `λ[#13 `@k #1]  -- Λ u. λ (tmu : t ~ Maybe u). λ (eqU : Eq u)
-                                                   -- eqMaybeU[u] eqU ▹ (t ~ Maybe u) → (t ~ Maybe u) → <Bool>
-                                              (#5 `@t #2 `@ #0) ▹ sym! (#1 -c> #2  -c> refl! #19))
-
-
-                   )
-    -- eqMaybe : ∀ u. Eq u → Maybe u → Maybe u → Bool
-    , .term (∀[★] (#9 `@k #0) -t> (#5 `@k #1) -t> (#6 `@k #2) -t> #15)
-     /-
-       eqMaybe := Λu. λ eu. λ mx. λ my.
-                      case mx of
-                        Nothing[u] → case my of
-                                          Nothing[u] → True
-                                          _ → False
-                        Just[u] → λ x. case my of
-                                          Nothing[u] → False
-                                          Just[u] → λ y. == x y
-     -/
-          (Λ[★] `λ[#9 `@k #0] `λ[#5 `@k #1] `λ[#6 `@k #2]
+    .inst 6 (Term.letterm ((∀[★] (#9 `@k #0) -t> (#5 `@k #1) -t> (#6 `@k #2) -t> #15))
+                          ((Λ[★] `λ[#9 `@k #0] `λ[#5 `@k #1] `λ[#6 `@k #2]
                 .ite (#6 `@t #3) #1
                      (.ite (#6 `@t #3) #0
                                #13    -- x = Nothing; y = Nothing
@@ -42,8 +23,15 @@ def MaybeBoolCtx : Ctx Term := [
                               (.ite (#6 `@t #4) #1 -- x = Just x'; y = Just y'
                                    (`λ[#4] ((#13 `@t #5 `@ #4) `@ #1 `@ #0))
                                     #14)))
-            #14)) -- catchall False
+                #14)))
+            (Λ[★] `λ[#10 `@k #0] -- Λt. λ(i : Eq t)
+                   .guard (#3 `@t #1) #0    --     EqMaybe[t] ← i
+                    (Λ[★] `λ[#2 ~ (#7 `@k #0)] `λ[#13 `@k #1]  -- Λ u. λ (tmu : t ~ Maybe u). λ (eqU : Eq u)
+                                                   -- eqMaybeU[u] eqU ▹ (t ~ Maybe u) → (t ~ Maybe u) → <Bool>
+                                              (#5 `@t #2 `@ #0) ▹ sym! (#1 -c> #2  -c> refl! #19))
 
+
+                   ))
 
 
 
@@ -58,12 +46,16 @@ def MaybeBoolCtx : Ctx Term := [
   , .datatype  (★ -k> ★)
 
 
-  , .inst 2 (Λ[★] `λ[#4 `@k #0] -- EqBool : Eq t
+  , .inst 1 (Term.letterm (#5 -t> (#6 -t> #7)) (`λ[#5] `λ[#6]
+        (Term.ite #5 #1 (Term.ite #5 #0 #5 #6)
+        (Term.ite #6 #1 (Term.ite #6 #0 #5 #6)
+          #6)))
+            (Λ[★] `λ[#4 `@k #0] -- EqBool : Eq t
                Term.guard (#3 `@t #1) -- EqBool[t]
                #0                     -- i
                 -- λ (tBool : t ~ Bool).  ==@Bool ▹ sym! (tBool -c> tBool -c> rfl Bool)
                (`λ[#1 ~ #8]
-                     (#3 ▹ sym! (#0 -c> (#1 -c> refl! #11)))))
+                     (#3 ▹ sym! (#0 -c> (#1 -c> refl! #11))))))
 
     -- ==@Bool : Bool → Bool → Bool
     /-   eqBool = λ x. λ y. case x of
@@ -74,11 +66,6 @@ def MaybeBoolCtx : Ctx Term := [
                                     True → False
                                     False → True
     -/
-  , .term (#5 -t> (#6 -t> #7))
-     (`λ[#5] `λ[#6]
-        (Term.ite #5 #1 (Term.ite #5 #0 #5 #6)
-        (Term.ite #6 #1 (Term.ite #6 #0 #5 #6)
-          #6)))
 
   -- EqBool : ∀ t. t ~ Bool → Eq t
   , .insttype (∀[★] (#0 ~ #5) -t> #3 `@k #1)
